Refactor

Finperm/Basic.lean
@@ -26,112 +26,69 @@ structure Finperm (n : Nat) where
 
 namespace Finperm
 
+open Function
 
-instance : GetElem (Finperm n) Nat Nat fun _ i => i < n where
-  getElem a i h := a.toVector[i]
+def get (a : Finperm n) (i : Fin n) : Fin n :=
+  ⟨a.toVector.get i, (a.getElem_invVector_getElem_toVector i.1 i.2).choose⟩
 
-@[simp, grind =]
-theorem getElem_mk (a b : Vector Nat n) {hab} {i : Nat} (hi : i < n) :
-  (Finperm.mk a b hab)[i]'hi = a[i]'hi := rfl
+theorem bijective_get (a : Finperm n) : a.get.Bijective := Injective.bijective_fin <|
+    fun i j h => Fin.ext <| by
+  have hget : ∀ i : Fin n, i = a.invVector[a.get i] :=
+    fun x => (a.getElem_invVector_getElem_toVector x.1 x.2).choose_spec.symm
+  rw [hget i, hget j, getElem_congr_idx h]
 
-@[simp, grind =]
-theorem getElem_toVector {i : Nat} {hi : i < n} {a : Finperm n} : a.toVector[i] = a[i] := rfl
-
-@[simp]
-theorem getElem_lt (a : Finperm n) (i : Nat) (hi : i < n) : a[i] < n :=
-  (a.getElem_invVector_getElem_toVector _ _).1
-
-grind_pattern getElem_lt => a[i]
-
-theorem getElem_ne (a : Finperm n) {i : Nat} {hi : i < n} : a[i] ≠ n := by grind
-
-grind_pattern getElem_ne => a[i]
-
-theorem eq_of_getElem_eq (a : Finperm n) (hi : i < n) (hj : j < n)
-    (hij : a[i] = a[j]) : i = j := by
-  grind [=_ getElem_toVector, getElem_invVector_getElem_toVector]
-
-@[simp, grind =] theorem getElem_inj (a : Finperm n) (hi : i < n) (hj : j < n) :
-    a[i] = a[j] ↔ i = j := by grind [eq_of_getElem_eq]
-
-theorem getElem_ne_iff (a : Finperm n) {i : Nat} (hi : i < n) {j : Nat} (hj : j < n) :
-    a[i] ≠ a[j] ↔ i ≠ j := by grind
+theorem injective_get (a : Finperm n) : a.get.Injective := a.bijective_get.injective
+theorem surjective_get (a : Finperm n) : a.get.Surjective := a.bijective_get.surjective
 
 theorem getElem_toVector_getElem_invVector {n} (a : Finperm n) (i : Nat) (hi : i < n) :
     ∃ hi' : a.invVector[i] < n, a.toVector[a.invVector[i]] = i := by
-  let f : Fin n → Fin n :=
-    fun x => ⟨a.toVector[x.1], (a.getElem_invVector_getElem_toVector x.1 x.2).choose⟩
-  have hspec : ∀ x : Fin n, a.invVector[a.toVector[x.1]]'(f x).2 = x.1 :=
-    fun x => (a.getElem_invVector_getElem_toVector x.1 x.2).choose_spec
-  have hfinj : f.Injective := fun x y hxy => Fin.ext <| (hspec x).symm.trans <|
-    (getElem_congr_idx (c := a.invVector) (w := (f x).2) (congrArg Fin.val hxy)).trans (hspec y)
-  obtain ⟨x, hx⟩ := hfinj.surjectiveOfFin ⟨i, hi⟩
-  have heq : a.toVector[x.1] = i := congrArg Fin.val hx
-  have hspec2 : a.invVector[i] = x.1 :=
-    (getElem_congr_idx (c := a.invVector) (w := (f x).2) heq).symm.trans (hspec x)
-  exact ⟨hspec2 ▸ x.2, (getElem_congr_idx (c := a.toVector) (w := hspec2 ▸ x.2) hspec2).trans heq⟩
-
-theorem getElem_surjective (a : Finperm n) (i : Nat) (hi : i < n) :
-    ∃ (j : Nat) (hj : j < n), a[j] = i := ⟨a.invVector[i], a.getElem_toVector_getElem_invVector _ _⟩
+  obtain ⟨j, _, hj⟩ := a.surjective_get ⟨i, hi⟩
+  have h := (a.getElem_invVector_getElem_toVector j j.isLt).choose_spec
+  exact ⟨h ▸ j.isLt, getElem_congr_idx h⟩
 
 instance : Inv (Finperm n) where
   inv a := ⟨a.invVector, a.toVector, a.getElem_toVector_getElem_invVector⟩
+
+theorem isEquiv_get_getInv (a : Finperm n) : a.get.IsEquiv a⁻¹.get :=
+    IsSplitting.isEquiv_fin <| fun _ => Fin.ext <| (a.getElem_toVector_getElem_invVector _ _).2
 
 @[simp, grind =]
 theorem inv_mk (a b : Vector Nat n) {hab} : (Finperm.mk a b hab)⁻¹ =
     Finperm.mk b a (Finperm.mk a b hab).getElem_toVector_getElem_invVector := rfl
 
 
-theorem getElem_inv_mk (a b : Vector Nat n) {hab} (hi : i < n) :
-  (Finperm.mk a b hab)⁻¹[i] = b[i] := by grind
+instance : GetElem (Finperm n) Nat Nat fun _ i => i < n where
+  getElem a i h := a.toVector[i]
+
+@[simp, grind =]
+theorem getElem_toVector {i : Nat} {hi : i < n} {a : Finperm n} : a.toVector[i] = a[i] := rfl
 
 @[simp, grind =]
 theorem getElem_invVector  (a : Finperm n) {i} (hi : i < n) : a.invVector[i] = a⁻¹[i] := rfl
 
-@[simp, grind =]
-theorem getElem_inv_getElem (a : Finperm n) {i} (hi : i < n) :
-    a⁻¹[a[i]] = i := (a.getElem_invVector_getElem_toVector _ _).2
+@[simp] theorem getElem_lt (a : Finperm n) (i : Nat) (hi : i < n) : a[i] < n :=
+  (a.getElem_invVector_getElem_toVector _ _).1
 
-@[simp, grind =]
-theorem getElem_getElem_inv (a : Finperm n) {i} (hi : i < n) :
-  a[a⁻¹[i]] = i := (a.getElem_toVector_getElem_invVector _ _).2
+grind_pattern getElem_lt => a[i]
 
-theorem eq_getElem_inv_iff (a : Finperm n) {i} (hi : i < n) (hj : j < n) :
-    i = a⁻¹[j] ↔ a[i] = j := by grind
+@[simp, grind =] theorem getElem_mk (a b : Vector Nat n) {hab} {i : Nat} (hi : i < n) :
+  (Finperm.mk a b hab)[i]'hi = a[i]'hi := rfl
 
-theorem ne_getElem_inv_iff (a : Finperm n) {i} (hi : i < n) (hj : j < n) :
-    i ≠ a⁻¹[j] ↔ a[i] ≠ j := by grind
+@[grind =>]
+theorem eq_of_getElem_eq (a : Finperm n) (hi : i < n) (hj : j < n)
+    (hij : a[i] = a[j]) : i = j := congrArg Fin.val (a.injective_get <| Fin.ext hij)
 
-theorem getElem_inv_eq_iff (a : Finperm n) {i} (hi : i < n) (hj : j < n) :
-    a⁻¹[i] = j ↔ i = a[j] := by grind
+@[simp] theorem getElem_eq_iff (a : Finperm n) (hi : i < n) (hj : j < n) :
+    a[i] = a[j] ↔ i = j := by grind
 
-theorem getElem_inv_ne_iff (a : Finperm n) {i} (hi : i < n) (hj : j < n) :
-    a⁻¹[i] ≠ j ↔ i ≠ a[j] := by grind
+@[simp, grind =] theorem getElem_getElem_inv (a : Finperm n) {i} (hi : i < n) :
+  a[a⁻¹[i]] = i := congrArg Fin.val (a.isEquiv_get_getInv.isSplitting_left _)
 
-theorem nodup_toVector (a : Finperm n) : a.toVector.Nodup := by
-  simp [Vector.nodup_iff_eq_of_getElem_eq]
-
-theorem nodup_invVector (a : Finperm n) : a.invVector.Nodup := by
-  simp [Vector.nodup_iff_eq_of_getElem_eq]
-
-@[grind =]
-theorem mem_toVector_iff_lt (a : Finperm n) {i : Nat} : i ∈ a.toVector ↔ i < n :=
-  a.toVector.mem_iff_getElem.trans ⟨by grind, a.getElem_surjective _⟩
-
-@[grind =]
-theorem mem_invVector_iff_lt (a : Finperm n) {i : Nat} : i ∈ a.invVector ↔ i < n :=
-  a.invVector.mem_iff_getElem.trans ⟨by grind, a⁻¹.getElem_surjective _⟩
-
-theorem mem_toVector_of_lt (a : Finperm n) : ∀ i < n, i ∈ a.toVector := by grind
-
-theorem mem_invVector_of_lt (a : Finperm n) : ∀ i < n, i ∈ a.invVector := by grind
-
-theorem lt_of_mem_toVector (a : Finperm n) : ∀ i ∈ a.toVector, i < n := by grind
-
-theorem lt_of_mem_invVector (a : Finperm n) : ∀ i ∈ a.invVector, i < n := by grind
+@[simp, grind =] theorem getElem_inv_getElem (a : Finperm n) {i} (hi : i < n) :
+  a⁻¹[a[i]] = i := congrArg Fin.val (a.isEquiv_get_getInv.isSplitting_right _)
 
 @[ext, grind ext]
-theorem ext (a b : Finperm n)  (h : ∀ (i : Nat) (hi : i < n), a[i] = b[i]) : a = b := by
+theorem ext (a b : Finperm n) (h : ∀ (i : Nat) (hi : i < n), a[i] = b[i]) : a = b := by
   suffices h : a.toVector = b.toVector ∧ a.invVector = b.invVector by grind [cases Finperm]
   grind
 
@@ -146,8 +103,48 @@ instance : Subsingleton (Finperm 0) where allEq a b := by grind
 
 instance : Subsingleton (Finperm 1) where allEq a b := by grind
 
+theorem getElem_ne_iff (a : Finperm n) {i : Nat} (hi : i < n) {j : Nat} (hj : j < n) :
+    a[i] ≠ a[j] ↔ i ≠ j := by grind
+
+theorem eq_getElem_inv_iff (a : Finperm n) {i} (hi : i < n) (hj : j < n) :
+    i = a⁻¹[j] ↔ a[i] = j := by grind
+
+theorem ne_getElem_inv_iff (a : Finperm n) {i} (hi : i < n) (hj : j < n) :
+    i ≠ a⁻¹[j] ↔ a[i] ≠ j := by grind
+
+theorem getElem_inv_eq_iff (a : Finperm n) {i} (hi : i < n) (hj : j < n) :
+    a⁻¹[i] = j ↔ i = a[j] := by grind
+
+theorem getElem_inv_ne_iff (a : Finperm n) {i} (hi : i < n) (hj : j < n) :
+    a⁻¹[i] ≠ j ↔ i ≠ a[j] := by grind
+
+theorem exists_getElem_eq_of_lt (a : Finperm n) (i : Nat) (hi : i < n) :
+    ∃ (j : Nat) (hj : j < n), a[j] = i := ⟨a.invVector[i], a.getElem_toVector_getElem_invVector _ _⟩
+
+theorem nodup_toVector (a : Finperm n) : a.toVector.Nodup := by
+  simp [Vector.nodup_iff_eq_of_getElem_eq]
+
+theorem nodup_invVector (a : Finperm n) : a.invVector.Nodup := by
+  simp [Vector.nodup_iff_eq_of_getElem_eq]
+
+@[grind =]
+theorem mem_toVector_iff_lt (a : Finperm n) {i : Nat} : i ∈ a.toVector ↔ i < n :=
+  a.toVector.mem_iff_getElem.trans ⟨by grind, a.exists_getElem_eq_of_lt _⟩
+
+@[grind =]
+theorem mem_invVector_iff_lt (a : Finperm n) {i : Nat} : i ∈ a.invVector ↔ i < n :=
+  a.invVector.mem_iff_getElem.trans ⟨by grind, a⁻¹.exists_getElem_eq_of_lt _⟩
+
+theorem mem_toVector_of_lt (a : Finperm n) : ∀ i < n, i ∈ a.toVector := by grind
+
+theorem mem_invVector_of_lt (a : Finperm n) : ∀ i < n, i ∈ a.invVector := by grind
+
+theorem lt_of_mem_toVector (a : Finperm n) : ∀ i ∈ a.toVector, i < n := by grind
+
+theorem lt_of_mem_invVector (a : Finperm n) : ∀ i ∈ a.invVector, i < n := by grind
+
 instance : One (Finperm n) where
-  one := Finperm.mk (Vector.range n) (Vector.range n) (by grind)
+  one := Finperm.mk (Vector.range n) (Vector.range n) (by simp)
 
 @[simp, grind =]
 theorem getElem_one {i : Nat} (hi : i < n) : (1 : Finperm n)[i] = i := Vector.getElem_range _
@@ -201,11 +198,11 @@ def toFinperm (v : Vector Nat n) (h : ∀ i < n, i ∈ v := by decide) : Finperm
     exact ⟨lt_of_lt_of_eq (List.idxOf_lt_length_of_mem (List.mem_of_getElem rfl))
     length_toList, List.getElem_idxOf _⟩
 
-theorem inv_toFinPerm (v : Vector Nat n) (h : ∀ i < n, i ∈ v) : (v.toFinperm h)⁻¹ =
-    (v.toFinperm h).nodup_invVector.toFinperm v (v.toFinperm h)⁻¹.getElem_lt := rfl
-
 theorem Nodup.inv_toFinPerm (v : Vector Nat n) (h₁ : v.Nodup) (h₂ : ∀ i (hi : i < n), v[i] < n) :
     (h₁.toFinperm v h₂)⁻¹ = v.toFinperm (h₁.toFinperm v h₂).mem_toVector_of_lt := rfl
+
+theorem inv_toFinPerm (v : Vector Nat n) (h : ∀ i < n, i ∈ v) : (v.toFinperm h)⁻¹ =
+    (v.toFinperm h).nodup_invVector.toFinperm v (v.toFinperm h)⁻¹.getElem_lt := rfl
 
 def shuffle (v : Vector α n) (a : Finperm n) : Vector α n := v.mapFinIdx fun i _ hi => v[a[i]]
 
@@ -216,6 +213,9 @@ def shuffle (v : Vector α n) (a : Finperm n) : Vector α n := v.mapFinIdx fun i
 theorem range_shuffle (a : Finperm n) :
     (Vector.range n).shuffle a = a.toVector := by grind
 
+theorem shuffle_range_inv :
+    (Vector.range n).shuffle a⁻¹ = a.invVector := by grind
+
 @[simp] theorem shuffle_one (v : Vector α n) :
     v.shuffle (1 : (Finperm n)) = v := by grind
 
@@ -224,9 +224,6 @@ theorem range_shuffle (a : Finperm n) :
 
 @[simp] theorem shuffle_shuffle_inv (v : Vector α n) (a : Finperm n) :
     (v.shuffle a).shuffle a⁻¹ = v := by grind
-
-theorem shuffle_range_inv :
-    (Vector.range n).shuffle a⁻¹ = a.invVector := by grind
 
 @[simp] theorem shuffle_mul (v : Vector α n) (a b : Finperm n) :
     v.shuffle (a * b) = (v.shuffle a).shuffle b := by grind
