Finperm/Function/Basic.lean
@@ -1,0 +1,80 @@
+/-
+Copyright (c) 2026 Kry10. All rights reserved.
+Released under Apache 2.0 license as described in the file LICENSE.
+Authors: Wrenna Robson
+-/
+module
+import Batteries.Tactic.Alias
+
+@[expose] public section
+
+namespace Function
+
+/-- A function is called bijective if it is both injective and surjective. -/
+def Bijective (f : α → β) :=
+  Injective f ∧ Surjective f
+
+protected theorem Bijective.injective : Bijective f → Injective f := And.left
+protected theorem Bijective.surjective : Bijective f → Surjective f := And.right
+
+theorem bijective_of_injective_of_surjective : Injective f → Surjective f → Bijective f :=
+  And.intro
+
+protected alias Injective.bijective_of_surjective := bijective_of_injective_of_surjective
+
+protected alias Surjective.bijective_of_injective := bijective_of_injective_of_surjective
+
+/-- A pair of functions `(f, g)` is a *splitting* (implicitly, of the identity) when `f` is a left
+inverse to`g`, i.e. `f ∘ g = id`. -/
+def IsSplitting (f : α → β) (g : β → α) := ∀ i, f (g i) = i
+
+theorem IsSplitting.comp_eq_id (h : IsSplitting f g) : f ∘ g = id := funext h
+
+theorem IsSplitting.injective : IsSplitting f g → Injective g := fun h i j hij =>
+  (h i).symm.trans <| (congrArg f hij).trans (h j)
+
+theorem IsSplitting.surjective : IsSplitting f g → Surjective f := fun h i => ⟨g i, h i⟩
+
+theorem isSplitting_of_isSplitting_of_injective :
+    IsSplitting f g → Injective f → IsSplitting g f := fun h => (· <| h <| f <| ·)
+
+theorem isSplitting_of_isSplitting_of_surjective :
+    IsSplitting f g → Surjective g → IsSplitting g f :=
+  fun h => (let ⟨y, hy⟩ := · ·; hy ▸ congrArg g (h y))
+
+alias IsSplitting.isSplitting_of_surjective := isSplitting_of_isSplitting_of_surjective
+alias IsSplitting.isSplitting_of_injective := isSplitting_of_isSplitting_of_injective
+alias Injective.isSplitting_of_isSplitting := isSplitting_of_isSplitting_of_injective
+alias Surjective.isSplitting_of_isSplitting := isSplitting_of_isSplitting_of_surjective
+
+/-- A pair of functions `(f, g)` form an equivalence when they are mutual two-sided inverses,
+i.e. `f ∘ g = id` and `g ∘ f = id`. -/
+def IsEquiv (f : α → β) (g : β → α) := IsSplitting f g ∧ IsSplitting g f
+
+theorem IsEquiv.symm : IsEquiv f g → IsEquiv g f := And.symm
+theorem isEquiv_comm : IsEquiv f g ↔ IsEquiv g f := And.comm
+
+protected theorem IsEquiv.isSplitting_left : IsEquiv f g → IsSplitting f g := And.left
+protected theorem IsEquiv.isSplitting_right : IsEquiv f g → IsSplitting g f := And.right
+
+theorem isEquiv_of_isSplitting_of_isSplitting :
+    IsSplitting f g → IsSplitting g f → IsEquiv f g := And.intro
+
+protected alias IsSplitting.isEquiv_of_isSplitting := isEquiv_of_isSplitting_of_isSplitting
+
+theorem isEquiv_of_isSplitting_of_surjective : IsSplitting f g → Surjective g ->
+    IsEquiv f g := fun hfg => hfg.isEquiv_of_isSplitting ∘ hfg.isSplitting_of_surjective
+
+theorem isEquiv_of_isSplitting_of_injective : IsSplitting f g → Injective f ->
+    IsEquiv f g := fun hfg => hfg.isEquiv_of_isSplitting ∘ hfg.isSplitting_of_injective
+
+alias IsSplitting.isEquiv_of_surjective := isEquiv_of_isSplitting_of_surjective
+alias Surjective.isEquiv_of_isSplitting := isEquiv_of_isSplitting_of_surjective
+alias IsSplitting.isEquiv_of_injective := isEquiv_of_isSplitting_of_injective
+alias Injective.isEquiv_of_isSplitting := isEquiv_of_isSplitting_of_injective
+
+theorem IsEquiv.bijective_right : IsEquiv f g → Bijective g :=
+  And.imp LeftInverse.injective RightInverse.surjective
+
+theorem IsEquiv.bijective_left : IsEquiv f g → Bijective f :=
+  IsEquiv.bijective_right ∘ And.symm
