Finperm/Function/Fin.lean
@@ -6,65 +6,66 @@ Authors: Wrenna Robson
 module
 
 public import Batteries.Data.Fin.Lemmas
-import Finperm.Function.Swap
+public import Finperm.Function.Swap
 
 @[expose] public section
 
 namespace Function
 
-theorem RightInverse.leftInverse_of_surjective {f : α → β} {g : β → α} :
-    RightInverse f g → Surjective f → LeftInverse f g :=
-  fun h hg x ↦ let ⟨y, hy⟩ := hg x; hy ▸ congrArg f (h y)
+open Fin in
+theorem Injective.bijective_of_ge_fin {f : Fin n → Fin m} (hf : f.Injective) (h : m ≤ n) :
+    f.Bijective ∧ n = m := by
+  induction m generalizing n with
+  | zero => exact ⟨⟨hf, (·.elim0)⟩, Nat.eq_zero_of_not_pos fun hf => (f ⟨0, hf⟩).elim0⟩
+  | succ m IH =>
+    rcases Nat.exists_eq_add_of_lt h with ⟨k, rfl⟩
+    let g := swapVal (last m) (f (last (m + k)))
+    let F (j : Fin (m + k)) : Fin m := ((g ∘ f) j.castSucc).castLT (val_lt_last <| by grind)
+    have hF : F.Injective := by grind [Function.Injective]
+    obtain ⟨hFbij, hmk⟩ := IH hF (Nat.le_add_right _ _)
+    have hgf : Surjective (g ∘ f) := by
+      apply Fin.lastCases
+      · exact ⟨last _, swapVal_apply_right _ _⟩
+      · intro i
+        rcases hFbij.surjective i with ⟨t, rfl⟩
+        exact ⟨t.castSucc, Fin.ext rfl⟩
+    exact ⟨⟨hf, fun a => (hgf (g a)).imp fun _ hx => swapVal_bijective.injective hx⟩, by omega⟩
+
+theorem Injective.bijective_fin {f : Fin n → Fin n} (hf : f.Injective) : f.Bijective :=
+  (hf.bijective_of_ge_fin (Nat.le_refl _)).1
+
+theorem Surjective.bijective_of_le_fin {f : Fin n → Fin m} (hf : f.Surjective)
+    (h : n ≤ m) : f.Bijective ∧ n = m := by
+  let g (y : Fin m) : Fin n := (hf y).choose
+  have hg : f.IsSplitting g := fun y => (hf y).choose_spec
+  obtain ⟨hgBij, hmn⟩ := hg.injective.bijective_of_ge_fin h
+  exact ⟨⟨(hg.isSplitting_of_surjective hgBij.surjective).injective, hf⟩, hmn.symm⟩
+
+theorem Surjective.bijective_fin {f : Fin n → Fin n} (hf : f.Surjective) : f.Bijective :=
+  (hf.bijective_of_le_fin (Nat.le_refl _)).1
+
+@[simp] theorem injective_iff_bijective_fin {f : Fin n → Fin n} : f.Injective ↔ f.Bijective :=
+  ⟨Injective.bijective_fin, Bijective.injective⟩
+
+@[simp] theorem surjective_iff_bijective_fin {f : Fin n → Fin n} : f.Surjective ↔ f.Bijective :=
+  ⟨Surjective.bijective_fin, Bijective.surjective⟩
+
+theorem IsSplitting.isSplitting_fin {f g : Fin n → Fin n} (h : f.IsSplitting g) :
+    g.IsSplitting f := h.isSplitting_of_surjective h.injective.bijective_fin.surjective
+
+theorem IsSplitting.isEquiv_fin {f g : Fin n → Fin n} (hf : f.IsSplitting g) : f.IsEquiv g :=
+  hf.isEquiv_of_injective hf.surjective.bijective_fin.injective
+
+@[simp] theorem isSplitting_iff_isEquiv_fin {f g : Fin n → Fin n} :
+    f.IsSplitting g ↔ f.IsEquiv g := (and_iff_left_of_imp IsSplitting.isSplitting_fin).symm
 
 def finInv (f : Fin n → Fin n) : Fin n → Fin n := fun i => (Fin.find? (f · == i)).getD i
 
-theorem apply_finInv_eq_of_apply_eq {f : Fin n → Fin n} (hf : f j = i) :
-    f (finInv f i) = i := by
-  have h : (Fin.find? (f · == i)).isSome := Fin.isSome_find?_of_eq_true (beq_of_eq hf)
-  rw [finInv, ← beq_iff_eq, ← Option.get_eq_getD (Fin.find? (f · == i)) (h := h),
-    Fin.get_find?_eq_true h]
-
-theorem Surjective.rightInverse_finInv {f : Fin n → Fin n} (hf : f.Surjective) :
-    (finInv f).RightInverse f := fun i => apply_finInv_eq_of_apply_eq (hf i).choose_spec
-
-theorem Injective.leftInverse_finInv {f : Fin n → Fin n} (hf : f.Injective) :
-    (finInv f).LeftInverse f := fun _ => hf (apply_finInv_eq_of_apply_eq rfl)
-
-theorem Surjective.injective_finInv {f : Fin n → Fin n} (hf : f.Surjective) :
-    (finInv f).Injective := hf.rightInverse_finInv.injective
-
-theorem Injective.surjective_finInv {f : Fin n → Fin n} (hf : f.Injective) :
-    (finInv f).Surjective := RightInverse.surjective hf.leftInverse_finInv
-
-open Fin in
-theorem Injective.surjectiveOfFin {f : Fin n → Fin n} (hf : f.Injective) : f.Surjective := by
-  induction n with
-  | zero => exact (·.elim0)
-  | succ n IH =>
-    let g := swapVal (last n) (f (last n))
-    have hgf : Surjective (g ∘ f) := by
-      apply Fin.lastCases
-      · exact ⟨last n, swapVal_apply_right _ _⟩
-      · intro i
-        let F (j : Fin n) : Fin n := ((g ∘ f) j.castSucc).castLT (val_lt_last <| by grind)
-        have hF : F.Injective := by grind [Function.Injective]
-        exact (IH hF i).imp' Fin.castSucc (fun _ => Fin.ext ∘ congrArg (@Fin.val n))
-    exact fun a => (hgf (g a)).imp fun _ hx => swapVal_injective hx
-
-theorem Injective.rightInverse_finInv {f : Fin n → Fin n} (hf : f.Injective) :
-    (finInv f).RightInverse f := hf.surjectiveOfFin.rightInverse_finInv
-
-theorem Surjective.surjective_finInv {f : Fin n → Fin n} (hf : f.Surjective) :
-    (finInv f).Surjective := hf.injective_finInv.surjectiveOfFin
-
-theorem Surjective.leftInverse_finInv {f : Fin n → Fin n} (hf : f.Surjective) :
-    (finInv f).LeftInverse f :=
-  hf.rightInverse_finInv.leftInverse_of_surjective hf.surjective_finInv
-
-theorem Surjective.injectiveOfFin {f : Fin n → Fin n} (hf : f.Surjective) : f.Injective :=
-  hf.leftInverse_finInv.injective
-
-theorem Injective.injective_finInv {f : Fin n → Fin n} (hf : f.Injective) :
-    (finInv f).Injective := hf.surjective_finInv.injectiveOfFin
+theorem Bijective.isEquiv_finInv {f : Fin n → Fin n} (hf : f.Bijective) :
+    f.IsEquiv (finInv f) := IsSplitting.isEquiv_fin <| fun i => by
+  have h : (Fin.find? (f · == i)).isSome :=
+    Fin.isSome_find?_of_eq_true (beq_of_eq (hf.surjective i).choose_spec)
+  exact eq_of_beq <| (congrArg (f · == i) (Option.get_eq_getD _).symm).trans
+    (Fin.get_find?_eq_true h)
 
 end Function
